CredibleCompilation/RefCompiler/Metatheory.lean
@@ -23,6 +23,8 @@ theorem SExpr.isSafe_of_safe (e : SExpr) (σ : Store) (am : ArrayMem)
     simp [SExpr.safe] at h; simp [SExpr.isSafe, ih h]
   | floatExp e ih =>
     simp [SExpr.safe] at h; simp [SExpr.isSafe, ih h]
+  | floatSqrt e ih =>
+    simp [SExpr.safe] at h; simp [SExpr.isSafe, ih h]
   | farrRead arr idx ih =>
     simp [SExpr.safe] at h; simp [SExpr.isSafe, ih h.1, decide_eq_true_eq, h.2]
 
